src/MicroSail/Symbolic/Sound.v
@@ -45,7 +45,7 @@ From MicroSail Require Import
      Syntax
      Tactics
      Symbolic.Mutator.
-From MicroSail Require
+From MicroSail Require Import
      SemiConcrete.Mutator
      SemiConcrete.Outcome
      SemiConcrete.Sound.
@@ -71,459 +71,471 @@ Module Soundness
 
     Import DynMutV1.
 
+    Global Instance inst_heap : Inst SymbolicHeap SCHeap :=
+      instantiate_list.
+    Global Instance instlaws_heap : InstLaws SymbolicHeap SCHeap.
+    Proof. apply instantiatelaws_list. Qed.
+
+    (* Relate two symbolic instances at different points during execution. This
+       essentially encodes a preorder on the total space { Σ & SymInstance Σ },
+       which encodes that ι2 is a future of ι1, i.e. it is derived by compatible
+       for existing variables and values for new universal variables. *)
+    Definition syminstance_rel {Σ1 Σ2} (ζ : Sub Σ1 Σ2) (ι1 : SymInstance Σ1) (ι2 : SymInstance Σ2) : Prop :=
+      inst ι2 ζ = ι1.
+
+    Lemma syminstance_rel_refl {Σ} (ι : SymInstance Σ) :
+      syminstance_rel (sub_id Σ) ι ι.
+    Proof. apply inst_sub_id. Qed.
+
+    Lemma syminstance_rel_snoc {Σ1 Σ2 x τ} (ζ : Sub Σ1 Σ2) (ι1 : SymInstance Σ1) ι2 :
+      forall t v,
+        syminstance_rel (env_snoc ζ (x,τ) t) (env_snoc ι1 (x,τ) v) ι2 <->
+        syminstance_rel ζ ι1 ι2 /\ v = inst ι2 t.
+    Proof.
+      unfold syminstance_rel. intros. split.
+      - cbn; intros.
+        now dependent elimination H.
+      - cbn; intros []; subst; now cbn.
+    Qed.
+
+    Lemma syminstance_rel_comp {Σ0 Σ1 Σ2} (ζ1 : Sub Σ0 Σ1) (ζ2 : Sub Σ1 Σ2)
+          (ι0 : SymInstance Σ0) (ι2 : SymInstance Σ2):
+      syminstance_rel (sub_comp ζ1 ζ2) ι0 ι2 <->
+      syminstance_rel ζ1 ι0 (inst ι2 ζ2).
+    Proof. unfold syminstance_rel. now rewrite <- inst_subst. Qed.
+
+    Lemma syminstance_rel_wk1 {Σ : NCtx 𝑺 Ty} {x τ} (ι : SymInstance Σ) (v : Lit τ) :
+      syminstance_rel sub_wk1 ι (ι ► ((x, τ) ↦ v)).
+    Proof. apply inst_sub_wk1. Qed.
+
+    (* A relation that links semi-concrete states with symbolic states. This
+       simply requires that when instantiating the symbolic state you get the
+       semi-concrete one (and the path-condition is true). Note that the
+       equality used in the heap instantiation requires the symbolic and the
+       semi-concrete executor to be in lock step with respect to the heap: i.e.
+       the symbolic executor and the semi-concrete executor need to end up with
+       a heap that has the same chunks in the same order. This can be relaxed
+       later to allow permutations or even some kind of semantic equivalence. *)
+    Definition represents {Γ Σ} (ι : SymInstance Σ) (s__sym : SymbolicState Γ Σ) (s__sc : SCState Γ) : Prop :=
+      inst                ι (symbolicstate_heap s__sym)       = scstate_heap s__sc /\
+      inst                ι (symbolicstate_localstore s__sym) = scstate_localstore s__sc /\
+      inst_pathcondition  ι (symbolicstate_pathcondition s__sym).
+
+    (* This is a preservation lemma for state representation. The symbolic
+       executor is allwed to add a formula (local assumption) to the
+       path-condition if it's true for the current instance ι. We only
+       need the -> direction I think. *)
+    Lemma represents_assume_formula {Γ Σ} (ι : SymInstance Σ) (s__sym : SymbolicState Γ Σ) (s__sc : SCState Γ) fml :
+      represents ι s__sym s__sc /\ inst_formula ι fml <->
+      represents ι (symbolicstate_assume_formula fml s__sym) s__sc.
+    Proof. unfold represents; destruct s__sym, s__sc; cbn; intuition. Qed.
+
+    Lemma represents_produce_chunk {Γ Σ} (ι : SymInstance Σ) (c : Chunk Σ)
+          (s__sym : SymbolicState Γ Σ) (s__sc : SCState Γ) :
+      represents ι s__sym s__sc <->
+      represents ι (symbolicstate_produce_chunk c s__sym) (scstate_produce_chunk (inst ι c) s__sc).
+    Proof.
+      unfold represents; destruct s__sym, s__sc; cbn - [inst].
+      change (inst ι (cons c ?h)) with (cons (inst ι c) (inst ι h)).
+      apply and_iff_compat_r.
+      split; intros; subst; auto.
+      now dependent elimination H.
+    Qed.
+
+    Lemma inst_subst_formula {Σ1 Σ2} (ι : SymInstance Σ2) (ζ : Sub Σ1 Σ2) (fml : Formula Σ1) :
+      inst_formula (inst ι ζ) fml <-> inst_formula ι (subst ζ fml).
+    Proof. destruct fml; cbn - [inst]; now rewrite !inst_subst. Qed.
+
+    Lemma inst_subst_pathcondition {Σ1 Σ2} (ι : SymInstance Σ2) (ζ : Sub Σ1 Σ2) (pc : PathCondition Σ1) :
+      inst_pathcondition (inst ι ζ) pc <-> inst_pathcondition ι (subst ζ pc).
+    Proof.
+      induction pc; cbn - [inst].
+      - reflexivity.
+      - rewrite inst_subst_formula.
+        apply and_iff_compat_l, IHpc.
+    Qed.
+
+    (* This is another preservation lemma. This one covers every state change in
+       the symbolic executor that is implemented via a universal variable
+       substitution, i.e. local equality assumptions that are substituted right
+       away and allocation of fresh universal variables. *)
+    Lemma represents_rel {Γ Σ0 Σ1} (ζ1 : Sub Σ0 Σ1) (ι0 : SymInstance Σ0) (ι1 : SymInstance Σ1) :
+      syminstance_rel ζ1 ι0 ι1 ->
+      forall (s__sym : SymbolicState Γ Σ0) (s__sc : SCState Γ),
+        represents ι0 s__sym s__sc <->
+        represents ι1 (subst ζ1 s__sym) s__sc.
+    Proof.
+      unfold syminstance_rel, represents; intros. subst.
+      destruct s__sym as [pc δ__sym h__sym], s__sc as [δ__sc h__sc];
+        cbn - [inst inst_pathcondition].
+      now rewrite !inst_subst, inst_subst_pathcondition.
+    Qed.
+
+    (* These should be kept abstract in the rest of the proof. If you need some
+       property, add a lemma above. *)
+    Local Opaque inst.
+    Local Opaque inst_chunk.
+    Local Opaque inst_heap.
+    Local Opaque inst_pathcondition.
+    Local Opaque instantiate_env.
+    Local Opaque instantiate_list.
+    Local Opaque represents.
+    Local Opaque symbolicstate_assume_formula.
+    Local Opaque symbolicstate_produce_chunk.
+
+    Definition scmut_wp {Γ1 Γ2 A}
+      (m : SCMut Γ1 Γ2 A)
+      (POST : A -> SCState Γ2 -> Prop)
+      (s1 : SCState Γ1) : Prop :=
+      outcome_satisfy (m s1) (fun r => POST (scmutres_value r) (scmutres_state r)).
+
+    Definition ResultProperty Γ A Σ :=
+      DynamicMutatorResult Γ A Σ -> Prop.
+
+    Definition dmutres_leq {Γ A Σ} `{Subst A} (r1 r2 : DynamicMutatorResult Γ A Σ) : Prop :=
+      match r1 , r2 with
+      | MkDynMutResult ζ1 a1 s1, MkDynMutResult ζ2 a2 s2 =>
+        exists ζ21, (ζ1 = sub_comp ζ2 ζ21 /\ a1 = subst ζ21 a2 /\ s1 = subst ζ21 s2)
+      end.
+
+    Global Instance dmutres_leq_preorder {Γ A Σ} {subA : Subst A} {subLA : SubstLaws A} : PreOrder (@dmutres_leq Γ A Σ subA).
+    Proof.
+      constructor.
+      - intros [Σ1 ζ1 a1 s1]. exists (sub_id _).
+        now rewrite sub_comp_id_right, ?subst_sub_id.
+      - intros [Σ1 ζ1 a1 s1] [Σ2 ζ2 a2 s2] [Σ3 ζ3 a3 s3].
+        unfold dmutres_leq; cbn; intros; destruct_conjs; subst.
+        exists (sub_comp H0 H). now rewrite ?sub_comp_assoc, ?subst_sub_comp.
+    Qed.
+
+    Definition resultprop_specialize {Γ A Σ1 Σ2} (ζ : Sub Σ1 Σ2) :
+      ResultProperty Γ A Σ1 -> ResultProperty Γ A Σ2 :=
+      fun p r => p (cosubst_dmutres ζ r).
+
+    Definition resultprop_downwards_closed {Γ A Σ} `{Subst A} (p : ResultProperty Γ A Σ) : Prop :=
+      forall (r1 r2 : DynamicMutatorResult Γ A Σ),
+        dmutres_leq r1 r2 -> p r2 -> p r1.
+
+    Definition StateProperty Γ A Σ :=
+      forall Σ1, Sub Σ Σ1 -> A Σ1 -> SymbolicState Γ Σ1 -> Prop.
+
+    Definition stateprop_specialize {Γ A Σ1 Σ2} (ζ : Sub Σ1 Σ2) (p: StateProperty Γ A Σ1) :
+      StateProperty Γ A Σ2 := fun Σ3 ζ3 => p Σ3 (sub_comp ζ ζ3).
+
+    Definition stateprop_impl {Γ A Σ} (P Q : StateProperty Γ A Σ) : Prop :=
+      forall Σ1 (ζ : Sub Σ Σ1) (a : A Σ1) (s : SymbolicState Γ Σ1),
+        P Σ1 ζ a s -> Q Σ1 ζ a s.
+
+    Definition stateprop_downwards_closed {Γ Σ A} `{Subst A} (p : StateProperty Γ A Σ) : Prop :=
+      forall Σ1 Σ2 (ζ1 : Sub Σ Σ1) (ζ2 : Sub Σ1 Σ2) (a1 : A Σ1) (s1 : SymbolicState Γ Σ1),
+        p Σ1 ζ1 a1 s1 ->
+        p Σ2 (sub_comp ζ1 ζ2) (subst ζ2 a1) (subst ζ2 s1).
+
+    Definition dmut_wp {Γ1 Γ2 Σ0 A}
+      (m : DynamicMutator Γ1 Γ2 A Σ0)
+      (POST : StateProperty Γ2 A Σ0)
+      (s1 : SymbolicState Γ1 Σ0) : Prop :=
+      forall Σ1 (ζ1 : Sub Σ0 Σ1),
+        outcome_satisfy
+          (m Σ1 ζ1 (subst ζ1 s1))
+          (fun '(@MkDynMutResult _ _ _ Σ2 ζ2 a2 s2) =>
+             POST Σ2 (sub_comp ζ1 ζ2) a2 s2).
+
+    Lemma dmut_wp_monotonic {Γ1 Γ2 Σ0 A} (m : DynamicMutator Γ1 Γ2 A Σ0)
+          (P Q : StateProperty Γ2 A Σ0) (HYP : stateprop_impl P Q) :
+      forall (s1 : SymbolicState Γ1 Σ0),
+        dmut_wp m P s1 -> dmut_wp m Q s1.
+    Proof.
+      unfold dmut_wp; cbn; intros s1 H Σ1 ζ1.
+      specialize (H Σ1 ζ1). revert H.
+      apply outcome_satisfy_monotonic.
+      intros [Σ2 ζ2 a2 s2]; cbn.
+      intuition.
+    Qed.
+
+    Definition stateprop_lift {Γ AT A Σ} {instA : Inst AT A} (ι : SymInstance Σ) (POST : A -> SCState Γ -> Prop) :
+      StateProperty Γ AT Σ :=
+      fun Σ1 ζ1 v1 s__sym1 =>
+        forall ι1 s__sc1,
+          syminstance_rel ζ1 ι ι1 ->
+          represents ι1 s__sym1 s__sc1 ->
+          POST (inst ι1 v1) s__sc1.
+
+    Lemma stateprop_lift_dcl {Γ AT A Σ} `{InstLaws AT A} (ι : SymInstance Σ) (POST : A -> SCState Γ -> Prop) :
+      stateprop_downwards_closed (stateprop_lift ι POST).
+    Proof.
+      unfold stateprop_downwards_closed, stateprop_lift; intros.
+      rewrite inst_subst.
+      apply syminstance_rel_comp in H4.
+      apply (H3 (inst ι1 ζ2) s__sc1).
+      - assumption.
+      - revert H5. now apply represents_rel.
+    Qed.
+
+    Definition approximates {Γ1 Γ2 AT A Σ} `{instA : Inst AT A} (ι : SymInstance Σ)
+               (dm : DynamicMutator Γ1 Γ2 AT Σ) (sm : SCMut Γ1 Γ2 A) : Prop :=
+      forall (s__sym : SymbolicState Γ1 Σ) (s__sc : SCState Γ1) (POST : A -> SCState Γ2 -> Prop),
+        represents ι s__sym s__sc ->
+        dmut_wp dm (stateprop_lift ι POST) s__sym ->
+        scmut_wp sm POST s__sc.
+
+    Lemma scmut_wp_demonic_binary {Γ1 Γ2 A} (sm1 sm2 : SCMut Γ1 Γ2 A) (s__sc : SCState Γ1) (POST : A -> SCState Γ2 -> Prop) :
+      scmut_wp (scmut_demonic_binary sm1 sm2) POST s__sc <-> scmut_wp sm1 POST s__sc /\ scmut_wp sm2 POST s__sc.
+    Proof. unfold scmut_wp, scmut_demonic_binary; cbn; intuition. Qed.
+
+    Lemma dmut_wp_demonic_binary {Γ1 Γ2 Σ A} (m1 m2 : DynamicMutator Γ1 Γ2 A Σ)
+      (POST : forall Σ', Sub Σ Σ' -> A Σ' -> SymbolicState Γ2 Σ' -> Prop) (s : SymbolicState Γ1 Σ) :
+        dmut_wp (dmut_demonic_binary m1 m2) POST s <->
+        dmut_wp m1 POST s /\ dmut_wp m2 POST s.
+    Proof. unfold dmut_wp, dmut_demonic_binary; cbn; intuition. Qed.
+
+    Lemma approximates_demonic_binary {Γ1 Γ2 Σ} (ι : SymInstance Σ)
+          (dm1 dm2 : DynamicMutator Γ1 Γ2 Unit Σ) (sm1 sm2 : SCMut Γ1 Γ2 unit) :
+      approximates ι dm1 sm1 ->
+      approximates ι dm2 sm2 ->
+      approximates ι (dmut_demonic_binary dm1 dm2) (scmut_demonic_binary sm1 sm2).
+    Proof.
+      intros H1 H2 ? ? ? H__s H.
+      apply scmut_wp_demonic_binary.
+      apply dmut_wp_demonic_binary in H.
+      split.
+      now apply (H1 _ _ _ H__s).
+      now apply (H2 _ _ _ H__s).
+    Qed.
+
+    Lemma scmut_wp_demonic {Γ1 Γ2 A B} (sm : B -> SCMut Γ1 Γ2 A) (s__sc : SCState Γ1) (POST : A -> SCState Γ2 -> Prop) :
+      scmut_wp (scmut_demonic sm) POST s__sc <-> forall v, scmut_wp (sm v) POST s__sc.
+    Proof. unfold scmut_wp, scmut_demonic; cbn; intuition. Qed.
+
+    Lemma dmut_wp_demonic {Γ1 Γ2 Σ A B} (m : B -> DynamicMutator Γ1 Γ2 A Σ)
+      (POST : StateProperty Γ2 A Σ) (s : SymbolicState Γ1 Σ) :
+        dmut_wp (dmut_demonic m) POST s <->
+        forall b, dmut_wp (m b) POST s.
+    Proof. unfold dmut_wp, dmut_demonic; cbn; intuition. Qed.
+
+    Lemma dmut_wp_produce_chunk {Γ Σ} (c : Chunk Σ) (s__sym : SymbolicState Γ Σ)
+          (POST : StateProperty Γ Unit Σ) (POST_dcl : stateprop_downwards_closed POST) :
+      dmut_wp (dmut_produce_chunk c) POST s__sym <->
+      POST Σ (sub_id Σ) tt (symbolicstate_produce_chunk c s__sym).
+    Proof.
+      split.
+      - intros dwp. specialize (dwp Σ (sub_id Σ)). cbn in dwp.
+        now rewrite ?sub_comp_id_left, ?subst_sub_id in dwp.
+      - intros ? ? ?. cbn.
+        replace (symbolicstate_produce_chunk (subst ζ1 c) (subst ζ1 s__sym))
+          with (subst ζ1 (symbolicstate_produce_chunk c s__sym)) by now destruct s__sym.
+        replace (sub_comp ζ1 (sub_id Σ1)) with (sub_comp (sub_id Σ) ζ1)
+          by now rewrite sub_comp_id_right, sub_comp_id_left.
+        now apply POST_dcl.
+    Qed.
+
+    Lemma dmut_produce_chunk_sound {Γ Σ} (ι : SymInstance Σ) (c : Chunk Σ) :
+      approximates
+        (Γ1 := Γ) (Γ2 := Γ) ι
+        (dmut_produce_chunk c)
+        (scmut_produce_chunk (inst ι c)).
+    Proof.
+      intros ? ? ? Hrep dwp. cbn.
+      apply dmut_wp_produce_chunk in dwp; auto using stateprop_lift_dcl.
+      apply (dwp ι); auto using syminstance_rel_refl.
+      now apply represents_produce_chunk.
+    Qed.
+
+    Lemma dmut_assume_term_sound {Γ Σ} (ι : SymInstance Σ) (b : Term Σ ty_bool) :
+      approximates
+        (Γ1 := Γ) (Γ2 := Γ) ι
+        (dmut_assume_term b)
+        (scmut_assume_term ι b).
+    Proof.
+      intros ? ? ? H__state H.
+      unfold dmut_wp, dmut_assume_term, dmut_assume_formula in H.
+      specialize (H Σ (sub_id Σ)).
+      change (sub_formula (sub_id Σ) (formula_bool b))
+        with (subst (sub_id Σ) (formula_bool b)) in H.
+      rewrite ?subst_sub_id in H.
+      unfold scmut_assume_term.
+      destruct (try_solve_formula (formula_bool b)) eqn:?.
+      - destruct (try_solve_formula_spec _ Heqo ι); clear Heqo.
+        + cbn in *.
+          rewrite i. cbn. apply (H ι).
+          rewrite sub_comp_id_left.
+          apply syminstance_rel_refl.
+          assumption.
+        + cbn in n. destruct (inst ι b); intuition.
+      - clear Heqo.
+        destruct (inst ι b) eqn:?; cbn.
+        * cbn in *.
+          apply (H ι).
+          rewrite sub_comp_id_left.
+          apply syminstance_rel_refl.
+          apply represents_assume_formula.
+          intuition.
+        * trivial.
+    Qed.
+
+    Opaque dmut_assume_term.
+
+    Definition dmut_wf {Γ1 Γ2 A Σ0} `{Subst A} (d : DynamicMutator Γ1 Γ2 A Σ0) : Prop :=
+      forall Σ1 Σ2 (ζ1 : Sub Σ0 Σ1) (ζ2 : Sub Σ1 Σ2) (s1 : SymbolicState Γ1 Σ1)
+             (POST : ResultProperty Γ2 A Σ1) (POST_dcl : resultprop_downwards_closed POST),
+        outcome_satisfy (d Σ1 ζ1 s1) POST ->
+        outcome_satisfy (d Σ2 (sub_comp ζ1 ζ2) (subst ζ2 s1)) (resultprop_specialize ζ2 POST).
+
+    Lemma dmut_wf_pure {Γ A Σ} {subA: Subst A} {sublA: SubstLaws A} (a : A Σ) :
+      dmut_wf (dmut_pure (Γ := Γ) a).
+    Proof.
+      unfold dmut_wf, resultprop_specialize; cbn; intros.
+      revert H.
+      apply POST_dcl.
+      unfold dmutres_leq.
+      exists ζ2; cbn.
+      rewrite sub_comp_id_right, sub_comp_id_left, subst_sub_comp.
+      intuition.
+    Qed.
+
+    Definition dmut_wf' {Γ1 Γ2 A Σ0} `{Subst A} (d : DynamicMutator Γ1 Γ2 A Σ0) : Prop :=
+      forall (POST : StateProperty Γ2 A Σ0) (POST_dcl : stateprop_downwards_closed POST)
+             (s : SymbolicState Γ1 Σ0) Σ1 (ζ : Sub Σ0 Σ1),
+        dmut_wp d POST s ->
+        dmut_wp (dmut_sub ζ d) (stateprop_specialize ζ POST) (subst ζ s).
+
+    Lemma dmut_wf'_pure {Γ A Σ} `{Subst A} (a : A Σ) :
+      dmut_wf' (dmut_pure (Γ := Γ) a).
+    Proof.
+      unfold dmut_wf', dmut_wp, dmut_sub, dmut_pure, stateprop_specialize; cbn; intros.
+      now rewrite <- sub_comp_assoc, <- subst_sub_comp.
+    Qed.
+
+    Lemma dmut_wf_equiv {Γ1 Γ2 A Σ0} `{Subst A} (d : DynamicMutator Γ1 Γ2 A Σ0) :
+      dmut_wf d <-> dmut_wf' d.
+    Proof.
+      unfold dmut_wf', dmut_wf, dmut_wp, dmut_sub; split; intros.
+      - specialize (H1 Σ2 (sub_comp ζ ζ1)). rewrite subst_sub_comp in H1.
+        refine (outcome_satisfy_monotonic _ _ H1).
+        clear. intros [Σ3 ζ3 r3].
+        unfold stateprop_specialize.
+        now rewrite sub_comp_assoc.
+      - admit.
+    Admitted.
+
+    Opaque subst.
+    Opaque sub_up1.
+    Opaque sub_snoc.
+    Opaque wk1.
+    Opaque SubstEnv.
+
+    Lemma dmut_wp_fresh {Γ Σ0 A x τ} `{Subst A}
+          (d : DynamicMutator Γ Γ A (Σ0 ▻ (x,τ))%ctx)
+          (POST : StateProperty Γ A Σ0)
+          (POST_dcl : stateprop_downwards_closed POST)
+          (s : SymbolicState Γ Σ0) (wfd : dmut_wf d) :
+      dmut_wp (dmut_fresh (x,τ) d) POST s <->
+      dmut_wp d (stateprop_specialize sub_wk1 POST) (subst sub_wk1 s).
+    Proof.
+      unfold dmut_wp, dmut_fresh; cbn; split; intros HYP ? ?.
+      - dependent elimination ζ1 as [@env_snoc Σ0 ζ1 _ v]; cbn in v.
+        rewrite <- subst_sub_comp, sub_comp_wk1_tail; cbn.
+        specialize (HYP Σ1 ζ1).
+        rewrite outcome_satisfy_map in HYP; cbn in *.
+        apply (@wfd _ Σ1 _ (env_snoc (sub_id _) (_,τ) v)) in HYP; clear wfd.
+        + change (wk1 (subst ζ1 s)) with (subst (sub_wk1 (b:=(x,τ))) (subst ζ1 s)) in HYP.
+          rewrite <- subst_sub_comp, <- sub_snoc_comp, sub_comp_id_right, sub_comp_wk1_tail in HYP.
+          cbn in HYP. rewrite subst_sub_id in HYP.
+          refine (outcome_satisfy_monotonic _ _ HYP).
+          intros [Σ2 ζ2 r2]. cbn. clear.
+          intuition.
+          rewrite <- (sub_comp_assoc sub_wk1), sub_comp_wk1_tail in H; cbn in H.
+          rewrite sub_comp_id_left in H.
+          unfold stateprop_specialize.
+          now rewrite <- sub_comp_assoc, sub_comp_wk1_tail.
+        + revert POST_dcl; clear.
+          unfold stateprop_downwards_closed, resultprop_downwards_closed.
+          intros ? [Σ2 ζ2 a2 s2] [Σ3 ζ3 a3 s3]; cbn.
+          intros [ζ12]; intuition. subst.
+          apply (POST_dcl _ _ _ ζ12) in H1.
+          now rewrite !sub_comp_assoc in H1.
+      - rewrite outcome_satisfy_map.
+        specialize (HYP (Σ1 ▻ (x,τ)) (sub_up1 ζ1)).
+        rewrite <- subst_sub_comp, sub_comp_wk1_comm in HYP.
+        change (wk1 (b := (x,τ)) (subst ζ1 s)) with (subst (sub_wk1 (b := (x,τ))) (subst ζ1 s)).
+        rewrite <- subst_sub_comp.
+        refine (outcome_satisfy_monotonic _ _ HYP).
+        intros [Σ2 ζ2 r2]. clear.
+        dependent elimination ζ2 as [@env_snoc Σ1 ζ2 _ t].
+        unfold stateprop_specialize.
+        now rewrite <- ?sub_comp_assoc, <- sub_comp_wk1_comm.
+    Qed.
+
+    Lemma dmut_fresh_sound {Γ Σ ς τ} (ι : SymInstance Σ)
+          (dm : DynamicMutator Γ Γ Unit (Σ ▻ (ς,τ))) (wfdm : dmut_wf dm)
+          (sm : Lit τ -> SCMut Γ Γ unit) :
+      (forall v, approximates (env_snoc ι _ v) dm (sm v)) ->
+      approximates ι
+        (dmut_fresh (ς,τ) dm)
+        (scmut_demonic sm).
+    Proof.
+      intros HYP.
+      unfold approximates; cbn.
+      intros ? ? ? H__state H.
+      apply scmut_wp_demonic. intros v.
+      apply (HYP v (subst sub_wk1 s__sym) s__sc POST).
+      - revert H__state. clear.
+        apply represents_rel.
+        apply syminstance_rel_wk1.
+      - apply (@dmut_wp_fresh Γ Σ Unit ς τ SubstUnit) in H.
+        + revert H; clear.
+          apply dmut_wp_monotonic; cbn; intros ? ? []; intros.
+          dependent elimination ζ as [@env_snoc Σ0 ζ _ t].
+          unfold stateprop_specialize in H.
+          rewrite sub_comp_wk1_tail in H; cbn in *.
+          intros ι1 s1 H0 H1.
+          apply H.
+          * now apply syminstance_rel_snoc in H0.
+          * assumption.
+        + apply stateprop_lift_dcl.
+        + assumption.
+    Qed.
+
+    Lemma dmut_produce_sound {Γ Σ} (asn : Assertion Σ) (ι : SymInstance Σ) :
+      approximates
+        (Γ1 := Γ) (Γ2 := Γ) ι
+        (dmut_produce asn)
+        (scmut_produce ι asn).
+    Proof.
+      induction asn; cbn.
+      - apply dmut_assume_term_sound.
+      - admit. (* Not implemented in SC. OOPS *)
+      - admit. (* destruct (Term_eqb t1 t2).
+        + apply dmut_pure_sound.
+        + apply dmut_fail_sound. *)
+      - apply dmut_produce_chunk_sound.
+      - enough
+          (approximates  (Γ1 := Γ) (Γ2 := Γ) ι
+             (dmut_demonic_binary
+                (dmut_bind_right (dmut_assume_term b)            (dmut_produce asn1))
+                (dmut_bind_right (dmut_assume_term (term_not b)) (dmut_produce asn2)))
+             (scmut_demonic_binary
+                (scmut_bind_right (scmut_assume_term ι b)            (scmut_produce ι asn1))
+                (scmut_bind_right (scmut_assume_term ι (term_not b)) (scmut_produce ι asn2)))) by admit.
+        apply approximates_demonic_binary.
+        + admit.
+        + admit.
+      - admit.
+      - admit.
+      - apply dmut_fresh_sound.
+        + admit.
+        + intros. apply IHasn.
+    Admitted.
+
+    Opaque dmut_wp.
+    Opaque scmut_wp.
+
     Section WithSemantics.
-
-      Global Instance inst_heap : Inst SymbolicHeap SCHeap :=
-        instantiate_list.
-      Global Instance instlaws_heap : InstLaws SymbolicHeap SCHeap.
-      Proof. apply instantiatelaws_list. Qed.
-
-      Definition represents {Γ Σ} (ι : SymInstance Σ) (s__sym : SymbolicState Γ Σ) (s__sc : SCState Γ) : Prop :=
-        inst                ι (symbolicstate_heap s__sym)       = scstate_heap s__sc /\
-        inst                ι (symbolicstate_localstore s__sym) = scstate_localstore s__sc /\
-        inst_pathcondition  ι (symbolicstate_pathcondition s__sym).
-
-      Definition syminstance_rel {Σ1 Σ2} (ζ : Sub Σ1 Σ2) (ι1 : SymInstance Σ1) (ι2 : SymInstance Σ2) : Prop :=
-        inst ι2 ζ = ι1.
-
-      Lemma syminstance_rel_refl {Σ} (ι : SymInstance Σ) :
-        syminstance_rel (sub_id Σ) ι ι.
-      Proof. apply inst_sub_id. Qed.
-
-      Lemma syminstance_rel_snoc {Σ1 Σ2 x τ} (ζ : Sub Σ1 Σ2) (ι1 : SymInstance Σ1) ι2 :
-        forall t v,
-          syminstance_rel ζ ι1 ι2 /\ v = inst ι2 t <->
-          syminstance_rel (env_snoc ζ (x,τ) t) (env_snoc ι1 (x,τ) v) ι2.
-      Proof.
-        unfold syminstance_rel. intros. split.
-        - cbn; intros []; subst; now cbn.
-        - cbn; intros.
-          now dependent elimination H.
-      Qed.
-
-      Local Opaque instantiate_env.
-      Local Opaque instantiate_list.
-      Local Opaque inst.
-
-      Lemma inst_subst_formula {Σ1 Σ2} (ι : SymInstance Σ2) (ζ : Sub Σ1 Σ2) (fml : Formula Σ1) :
-        inst_formula (inst ι ζ) fml <-> inst_formula ι (subst ζ fml).
-      Proof. destruct fml; cbn; now rewrite !inst_subst. Qed.
-
-      Lemma inst_subst_pathcondition {Σ1 Σ2} (ι : SymInstance Σ2) (ζ : Sub Σ1 Σ2) (pc : PathCondition Σ1) :
-        inst_pathcondition (inst ι ζ) pc <-> inst_pathcondition ι (subst ζ pc).
-      Proof.
-        induction pc; cbn.
-        - reflexivity.
-        - rewrite inst_subst_formula.
-          apply and_iff_compat_l, IHpc.
-      Qed.
-
-      Local Opaque inst_pathcondition.
-
-      Lemma represents_rel {Γ Σ} (ι : SymInstance Σ) (s__sym : SymbolicState Γ Σ) (s__sc : SCState Γ) :
-        forall Σ1 (ζ : Sub Σ Σ1) (ι2 : SymInstance Σ1),
-          syminstance_rel ζ ι ι2 ->
-          represents ι s__sym s__sc ->
-          represents ι2 (subst ζ s__sym) s__sc.
-      Proof.
-        unfold syminstance_rel, represents.
-        destruct s__sym as [pc δ__sym h__sym], s__sc as [δ__sc h__sc]; cbn.
-        intros ? ? ? <-.
-        now rewrite !inst_subst, inst_subst_pathcondition.
-      Qed.
-
-      Definition scmut_wp {Γ1 Γ2 A}
-        (m : SCMut Γ1 Γ2 A)
-        (POST : A -> SCState Γ2 -> Prop)
-        (s1 : SCState Γ1) : Prop :=
-        SemiConcrete.Outcome.outcome_satisfy (m s1) (fun r => POST (scmutres_value r) (scmutres_state r)).
-
-      Definition dmut_wp {Γ1 Γ2 Σ0 A}
-        (m : DynamicMutator Γ1 Γ2 A Σ0)
-        (POST : forall Σ1, Sub Σ0 Σ1 -> A Σ1 -> SymbolicState Γ2 Σ1 -> Prop)
-        (s1 : SymbolicState Γ1 Σ0) : Prop :=
-        forall Σ1 (ζ1 : Sub Σ0 Σ1),
-          SemiConcrete.Outcome.outcome_satisfy
-            (m Σ1 ζ1 (subst ζ1 s1))
-            (fun '(@MkDynMutResult _ _ _ Σ2 ζ2 a2 s2) =>
-               POST Σ2 (sub_comp ζ1 ζ2) a2 s2).
-
-      Lemma dmut_wp_monotonic {Γ1 Γ2 Σ0 A} (m : DynamicMutator Γ1 Γ2 A Σ0)
-            (POST1 POST2 : forall Σ1, Sub Σ0 Σ1 -> A Σ1 -> SymbolicState Γ2 Σ1 -> Prop)
-            (HYP : forall Σ1 (ζ : Sub Σ0 Σ1) (a : A Σ1) (s : SymbolicState Γ2 Σ1),
-                POST1 Σ1 ζ a s -> POST2 Σ1 ζ a s) (s1 : SymbolicState Γ1 Σ0) :
-        dmut_wp m POST1 s1 -> dmut_wp m POST2 s1.
-      Proof.
-        unfold dmut_wp; cbn; intros H Σ1 ζ1.
-        specialize (H Σ1 ζ1). revert H.
-        apply SemiConcrete.Outcome.outcome_satisfy_monotonic.
-        intros [Σ2 ζ2 a2 s2]; cbn.
-        intuition.
-      Qed.
-
-      Definition approximates {Γ1 Γ2 Σ} (ι : SymInstance Σ) (dm : DynamicMutator Γ1 Γ2 Unit Σ) (sm : SCMut Γ1 Γ2 unit) : Prop :=
-        forall (s__sym : SymbolicState Γ1 Σ) (s__sc : SCState Γ1) (POST : unit -> SCState Γ2 -> Prop),
-          represents ι s__sym s__sc ->
-          dmut_wp
-            dm
-            (fun Σ1 ζ1 v1 s__sym1 =>
-               forall ι1 s__sc1,
-                 syminstance_rel ζ1 ι ι1 ->
-                 represents ι1 s__sym1 s__sc1 ->
-                 POST v1 s__sc1)
-            s__sym ->
-          scmut_wp sm POST s__sc.
-
-      Lemma scmut_wp_demonic_binary {Γ1 Γ2 A} (sm1 sm2 : SCMut Γ1 Γ2 A) (s__sc : SCState Γ1) (POST : A -> SCState Γ2 -> Prop) :
-        scmut_wp (scmut_demonic_binary sm1 sm2) POST s__sc <-> scmut_wp sm1 POST s__sc /\ scmut_wp sm2 POST s__sc.
-      Proof. unfold scmut_wp, scmut_demonic_binary; cbn; intuition. Qed.
-
-      Lemma dmut_wp_demonic_binary {Γ1 Γ2 Σ A} (m1 m2 : DynamicMutator Γ1 Γ2 A Σ)
-        (POST : forall Σ', Sub Σ Σ' -> A Σ' -> SymbolicState Γ2 Σ' -> Prop) (s : SymbolicState Γ1 Σ) :
-          dmut_wp (dmut_demonic_binary m1 m2) POST s <->
-          dmut_wp m1 POST s /\ dmut_wp m2 POST s.
-      Proof. unfold dmut_wp, dmut_demonic_binary; cbn; intuition. Qed.
-
-      Lemma approximates_demonic_binary {Γ1 Γ2 Σ} (ι : SymInstance Σ)
-            (dm1 dm2 : DynamicMutator Γ1 Γ2 Unit Σ) (sm1 sm2 : SCMut Γ1 Γ2 unit) :
-        approximates ι dm1 sm1 ->
-        approximates ι dm2 sm2 ->
-        approximates ι (dmut_demonic_binary dm1 dm2) (scmut_demonic_binary sm1 sm2).
-      Proof.
-        intros H1 H2 ? ? ? H__s H.
-        apply scmut_wp_demonic_binary.
-        apply dmut_wp_demonic_binary in H.
-        split.
-        now apply (H1 _ _ _ H__s).
-        now apply (H2 _ _ _ H__s).
-      Qed.
-
-      Lemma scmut_wp_demonic {Γ1 Γ2 A B} (sm : B -> SCMut Γ1 Γ2 A) (s__sc : SCState Γ1) (POST : A -> SCState Γ2 -> Prop) :
-        scmut_wp (scmut_demonic sm) POST s__sc <-> forall v, scmut_wp (sm v) POST s__sc.
-      Proof. unfold scmut_wp, scmut_demonic; cbn; intuition. Qed.
-
-      Lemma dmut_wp_demonic {Γ1 Γ2 Σ A B} (m : B -> DynamicMutator Γ1 Γ2 A Σ)
-        (POST : forall Σ', Sub Σ Σ' -> A Σ' -> SymbolicState Γ2 Σ' -> Prop) (s : SymbolicState Γ1 Σ) :
-          dmut_wp (dmut_demonic m) POST s <->
-          forall b, dmut_wp (m b) POST s.
-      Proof. unfold dmut_wp, dmut_demonic; cbn; intuition. Qed.
-
-      Lemma dmut_produce_chunk_sound {Γ Σ} (ι : SymInstance Σ) (c : Chunk Σ) :
-        approximates
-          (Γ1 := Γ) (Γ2 := Γ) ι
-          (dmut_produce_chunk c)
-          (scmut_produce_chunk (inst ι c)).
-      Proof.
-        intros [pc δ__sym h__sym] [δ__sc h__sc] ? (H__h & H__δ & H__pc); cbn in *.
-        intros; destruct_conjs.
-        specialize (H Σ (sub_id Σ)). cbn in H.
-        apply (H ι); clear H.
-        rewrite sub_comp_id_left.
-        apply syminstance_rel_refl.
-        unfold represents; cbn.
-        subst; now rewrite ?subst_sub_id.
-      Qed.
-
-      Local Transparent inst_pathcondition.
-
-      Lemma dmut_assume_term_sound {Γ Σ} (ι : SymInstance Σ) (b : Term Σ ty_bool) :
-        approximates
-          (Γ1 := Γ) (Γ2 := Γ) ι
-          (dmut_assume_term b)
-          (scmut_assume_term ι b).
-      Proof.
-        intros ? ? ? H__state H.
-        unfold dmut_wp, dmut_assume_term, dmut_assume_formula in H.
-        specialize (H Σ (sub_id Σ)).
-        change (sub_formula (sub_id Σ) (formula_bool b))
-          with (subst (sub_id Σ) (formula_bool b)) in H.
-        rewrite ?subst_sub_id in H.
-        unfold scmut_assume_term.
-        destruct (try_solve_formula (formula_bool b)) eqn:?.
-        - destruct (try_solve_formula_spec _ Heqo ι); clear Heqo.
-          + cbn in *.
-            rewrite i. cbn. apply (H ι).
-            rewrite sub_comp_id_left.
-            apply syminstance_rel_refl.
-            assumption.
-          + cbn in n. destruct (inst ι b); intuition.
-        - clear Heqo.
-          destruct (inst ι b) eqn:?; cbn.
-          * cbn in *.
-            apply (H ι).
-            rewrite sub_comp_id_left.
-            apply syminstance_rel_refl.
-            revert H__state Heqy. clear.
-            unfold represents; destruct s__sym;
-              cbn; intuition.
-          * trivial.
-      Qed.
-
-      Opaque dmut_assume_term.
-
-      Definition dmutres_geq {Γ A Σ} `{Subst A} (r1 r2 : DynamicMutatorResult Γ A Σ) : Prop :=
-        match r1 , r2 with
-        | MkDynMutResult ζ1 a1 s1, MkDynMutResult ζ2 a2 s2 =>
-          exists ζ12, (ζ2 = sub_comp ζ1 ζ12 /\ a2 = subst ζ12 a1 /\ s2 = subst ζ12 s1)
-        end.
-
-      Definition dmutres_pred_monotonic {Γ A Σ} `{Subst A} (p : DynamicMutatorResult Γ A Σ -> Prop) : Prop :=
-        forall (r1 r2 : DynamicMutatorResult Γ A Σ),
-          dmutres_geq r1 r2 -> p r1 -> p r2.
-
-      Definition dmutres_sub {Γ A Σ1 Σ2} (ζ : Sub Σ1 Σ2) (r : DynamicMutatorResult Γ A Σ2) :
-        DynamicMutatorResult Γ A Σ1 :=
-        match r with
-        | @MkDynMutResult _ _ _ Σ3 ζ3 a3 s3 =>
-          @MkDynMutResult _ _ _ Σ3 (sub_comp ζ ζ3) a3 s3
-        end.
-
-      Definition substpred {Γ A Σ1 Σ2} (ζ : Sub Σ1 Σ2) :
-        (DynamicMutatorResult Γ A Σ1 -> Prop) ->
-        (DynamicMutatorResult Γ A Σ2 -> Prop) :=
-        fun p r => p (dmutres_sub ζ r).
-
-      Definition dmut_wf {Γ1 Γ2 A Σ0} `{Subst A} (d : DynamicMutator Γ1 Γ2 A Σ0) : Prop :=
-        forall Σ1 Σ2 (ζ1 : Sub Σ0 Σ1) (ζ2 : Sub Σ1 Σ2) (s1 : SymbolicState Γ1 Σ1)
-               (POST : DynamicMutatorResult Γ2 A Σ1 -> Prop) (POST_mon : dmutres_pred_monotonic POST),
-          SemiConcrete.Outcome.outcome_satisfy (d Σ1 ζ1 s1) POST ->
-          SemiConcrete.Outcome.outcome_satisfy (d Σ2 (sub_comp ζ1 ζ2) (subst ζ2 s1)) (substpred ζ2 POST).
-
-      Lemma dmut_wf_pure {Γ A Σ} {subA: Subst A} {sublA: SubstLaws A} (a : A Σ) :
-        dmut_wf (dmut_pure (Γ := Γ) a).
-      Proof.
-        unfold dmut_wf, substpred; cbn; intros.
-        revert H.
-        apply POST_mon.
-        unfold dmutres_geq.
-        exists ζ2; cbn.
-        fold (sub_comp ζ1 ζ2).
-        rewrite sub_comp_id_right, sub_comp_id_left, subst_sub_comp.
-        intuition.
-      Qed.
-
-      Definition dmut_pred_monotonic {Γ Σ0 A} `{Subst A} (p : forall Σ1, Sub Σ0 Σ1 -> A Σ1 -> SymbolicState Γ Σ1 -> Prop) : Prop :=
-        forall Σ1 Σ2 (ζ1 : Sub Σ0 Σ1) (ζ2 : Sub Σ1 Σ2) (a1 : A Σ1) (s1 : SymbolicState Γ _),
-          p Σ1 ζ1 a1 s1 ->
-          p Σ2 (sub_comp ζ1 ζ2) (subst ζ2 a1) (subst ζ2 s1).
-
-      Definition dmut_wf' {Γ1 Γ2 A Σ0} `{Subst A} (d : DynamicMutator Γ1 Γ2 A Σ0) : Prop :=
-        forall (POST : forall Σ1, Sub Σ0 Σ1 -> A Σ1 -> SymbolicState Γ2 Σ1 -> Prop)
-               (POST_mon : dmut_pred_monotonic POST)
-               (s : SymbolicState Γ1 Σ0) Σ1 (ζ : Sub Σ0 Σ1),
-          dmut_wp d POST s ->
-          dmut_wp (dmut_sub ζ d) (fun Σ2 ζ2 => POST Σ2 (sub_comp ζ ζ2)) (subst ζ s).
-
-      Lemma dmut_wf'_pure {Γ A Σ} `{Subst A} (a : A Σ) :
-        dmut_wf' (dmut_pure (Γ := Γ) a).
-      Proof.
-        unfold dmut_wf', dmut_wp, dmut_sub, dmut_pure; cbn; intros.
-        now rewrite <- sub_comp_assoc, <- subst_sub_comp.
-      Qed.
-
-      Opaque subst.
-      Opaque sub_up1.
-      Opaque sub_snoc.
-      Opaque wk1.
-      Opaque SubstEnv.
-
-      Lemma dmut_wp_fresh {Γ Σ0 A x τ} `{Subst A}
-            (d : DynamicMutator Γ Γ A (Σ0 ▻ (x,τ))%ctx)
-            (POST : forall Σ1, Sub Σ0 Σ1 -> A Σ1 -> SymbolicState Γ Σ1 -> Prop)
-            (POST_mon : dmut_pred_monotonic POST)
-            (s : SymbolicState Γ Σ0) (wfd : dmut_wf d) :
-        dmut_wp (dmut_fresh (x,τ) d) POST s <->
-        dmut_wp d (fun Σ1 ζ1 a1 s1 => POST Σ1 (sub_comp sub_wk1 ζ1) a1 s1) (subst sub_wk1 s).
-      Proof.
-        unfold dmut_wp, dmut_fresh; cbn; split; intros HYP ? ?.
-        - dependent elimination ζ1 as [@env_snoc Σ0 ζ1 _ v]; cbn in v.
-          rewrite <- subst_sub_comp, sub_comp_wk1_tail; cbn.
-          specialize (HYP Σ1 ζ1).
-          rewrite SemiConcrete.Outcome.outcome_satisfy_map in HYP; cbn in *.
-          eapply (@wfd _ Σ1 _ (env_snoc (sub_id _) (_,τ) v)) in HYP; clear wfd.
-          + change (wk1 (subst ζ1 s)) with (subst (sub_wk1 (b:=(x,τ))) (subst ζ1 s)) in HYP.
-            rewrite <- subst_sub_comp, <- sub_snoc_comp, sub_comp_id_right, sub_comp_wk1_tail in HYP.
-            cbn in HYP. rewrite subst_sub_id in HYP.
-            refine (SemiConcrete.Outcome.outcome_satisfy_monotonic _ _ HYP).
-            intros [Σ2 ζ2 r2]. cbn. clear.
-            intuition.
-            rewrite <- sub_comp_assoc, sub_comp_wk1_tail; cbn.
-            rewrite <- (sub_comp_assoc sub_wk1), sub_comp_wk1_tail in H; cbn in H.
-            now rewrite sub_comp_id_left in H.
-          + revert POST_mon; clear.
-            unfold dmutres_pred_monotonic.
-            intros ? [Σ2 ζ2 a2 s2] [Σ3 ζ3 a3 s3]; cbn.
-            intros [ζ12]; intuition. subst.
-            apply (POST_mon _ _ _ ζ12) in H1.
-            now rewrite !sub_comp_assoc in H1.
-        - rewrite SemiConcrete.Outcome.outcome_satisfy_map.
-          specialize (HYP (Σ1 ▻ (x,τ)) (sub_up1 ζ1)).
-          rewrite <- subst_sub_comp, sub_comp_wk1_comm in HYP.
-          change (wk1 (b := (x,τ)) (subst ζ1 s)) with (subst (sub_wk1 (b := (x,τ))) (subst ζ1 s)).
-          rewrite <- subst_sub_comp.
-          refine (SemiConcrete.Outcome.outcome_satisfy_monotonic _ _ HYP).
-          intros [Σ2 ζ2 r2]. clear.
-          dependent elimination ζ2 as [@env_snoc Σ1 ζ2 _ t].
-          now rewrite <- ?sub_comp_assoc, <- sub_comp_wk1_comm.
-      Qed.
-
-      (* Lemma dmut_wp_fresh' {Γ Σ0 A x τ} *)
-      (*       (d : DynamicMutator Γ Γ A (Σ0 ▻ (x,τ))%ctx) (wfd : dmut_wf d) *)
-      (*       (POST : forall Σ1, Sub Σ0 Σ1 -> A Σ1 -> SymbolicState Γ Σ1 -> Prop) *)
-      (*       (s : SymbolicState Γ Σ0) : *)
-      (*   dmut_wp (dmut_fresh (x,τ) d) POST s <-> *)
-      (*   forall v, *)
-      (*     dmut_wp (dmut_sub (env_snoc (sub_id Σ0) (x,τ) (term_lit τ v)) d) POST s. *)
-      (* Proof. *)
-      (*   unfold dmut_wp, dmut_fresh, dmut_sub; cbn. split; intro HYP. *)
-      (*   - intros. *)
-      (*     specialize (HYP Σ1 ζ1). *)
-      (*     rewrite outcome_satisfy_map in HYP; cbn in *. *)
-      (*     admit. *)
-      (*   - intros ? ?. *)
-      (*     rewrite outcome_satisfy_map. *)
-      (* Admitted. *)
-
-      (* Lemma dmut_wp_fresh_demonic {Γ Σ A x τ} *)
-      (*       (d__d : Lit τ -> DynamicMutator Γ Γ A Σ) *)
-      (*       (d__f : DynamicMutator Γ Γ A (Σ ▻ (x,τ))%ctx) : *)
-      (*   (forall v POST s, *)
-      (*       dmut_wp (d__d v) POST s <-> *)
-      (*       dmut_wp *)
-      (*         (dmut_sub (env_snoc (sub_id Σ) (x,τ) (term_lit τ v)) d__f) POST s) -> *)
-      (*   (forall *)
-      (*       (POST : forall Σ', Sub Σ Σ' -> A Σ' -> SymbolicState Γ Σ' -> Prop) *)
-      (*       (s : SymbolicState Γ Σ), *)
-      (*       dmut_wp (dmut_fresh (x,τ) d__f) POST s <-> *)
-      (*       dmut_wp (dmut_demonic d__d) POST s). *)
-      (* Proof. *)
-      (*   intros; split; intro HYP. *)
-      (*   - apply dmut_wp_demonic. intros. *)
-      (*     apply H. clear H. revert HYP. clear. *)
-      (*     unfold dmut_wp, dmut_fresh, dmut_sub; cbn; intros. *)
-      (*     specialize (HYP Σ1 ζ1). *)
-      (*     rewrite outcome_satisfy_map in HYP. *)
-      (* Admitted. *)
-
-      Local Opaque inst_pathcondition.
-      Local Transparent subst.
-
-      Lemma dmut_fresh_sound {Γ Σ ς τ} (ι : SymInstance Σ)
-            (dm : DynamicMutator Γ Γ Unit (Σ ▻ (ς,τ))) (wfdm : dmut_wf dm)
-            (sm : Lit τ -> SCMut Γ Γ unit) :
-        (forall v, approximates (env_snoc ι _ v) dm (sm v)) ->
-        approximates ι
-          (dmut_fresh (ς,τ) dm)
-          (scmut_demonic sm).
-      Proof.
-        intros HYP.
-        unfold approximates; cbn.
-        intros ? ? ? H__state H.
-        apply scmut_wp_demonic. intros v.
-        apply (HYP v (subst sub_wk1 s__sym) s__sc POST).
-        - revert H__state. clear.
-          destruct s__sym, s__sc; unfold represents; cbn.
-          intros; destruct_conjs; repeat split.
-          + now rewrite inst_subst, inst_sub_wk1.
-          + now rewrite inst_subst, inst_sub_wk1.
-          + now rewrite <- inst_subst_pathcondition, inst_sub_wk1.
-        - (* unfold dmut_wp, dmut_fresh in *. *)
-          (* intros ? ?. *)
-          (* dependent elimination ζ1 as [@env_snoc Σ ζ1 _ v]. cbn in v. *)
-          (* specialize (H Σ1 ζ1). *)
-          (* rewrite outcome_satisfy_map in H. *)
-          apply (@dmut_wp_fresh Γ Σ Unit ς τ SubstUnit) in H.
-          + revert H; clear.
-            apply dmut_wp_monotonic; cbn; intros.
-            dependent elimination ζ as [@env_snoc Σ0 ζ _ t]. cbn in t.
-            apply syminstance_rel_snoc in H0.
-            refine (H _ _ _ H1).
-            rewrite sub_comp_wk1_tail; cbn.
-            apply H0.
-          + clear. unfold dmut_pred_monotonic; intros. destruct a1; cbn.
-            unfold syminstance_rel in H0. subst.
-            apply (H (inst ι1 ζ2) s__sc1).
-            * unfold syminstance_rel.
-              now rewrite <- inst_subst.
-            * revert H1; clear.
-              destruct s1 as [pc1 δ__sym1 h__sym1]; cbn.
-              destruct s__sc1 as [δ__sc1 h__sc1].
-              unfold represents; cbn.
-              now rewrite !inst_subst, inst_subst_pathcondition.
-          + exact wfdm.
-      Qed.
-
-      Lemma dmut_produce_sound {Γ Σ} (asn : Assertion Σ) (ι : SymInstance Σ) :
-        approximates
-          (Γ1 := Γ) (Γ2 := Γ) ι
-          (dmut_produce asn)
-          (scmut_produce ι asn).
-      Proof.
-        induction asn; cbn.
-        - apply dmut_assume_term_sound.
-        - admit. (* Not implemented in SC. OOPS *)
-        - admit. (* destruct (Term_eqb t1 t2).
-          + apply dmut_pure_sound.
-          + apply dmut_fail_sound. *)
-        - apply dmut_produce_chunk_sound.
-        - enough
-            (approximates  (Γ1 := Γ) (Γ2 := Γ) ι
-               (dmut_demonic_binary
-                  (dmut_bind_right (dmut_assume_term b)            (dmut_produce asn1))
-                  (dmut_bind_right (dmut_assume_term (term_not b)) (dmut_produce asn2)))
-               (scmut_demonic_binary
-                  (scmut_bind_right (scmut_assume_term ι b)            (scmut_produce ι asn1))
-                  (scmut_bind_right (scmut_assume_term ι (term_not b)) (scmut_produce ι asn2)))) by admit.
-          apply approximates_demonic_binary.
-          + admit.
-          + admit.
-        - admit.
-        - admit.
-        - apply dmut_fresh_sound.
-          + admit.
-          + intros. apply IHasn.
-      Admitted.
-
-      Opaque dmut_wp.
-      Opaque scmut_wp.
 
       Context `{HL: IHeaplet L} {SLL: ISepLogicLaws L}.
 
       Definition interpret_heap {Σ} (ι : SymInstance Σ) (h : SymbolicHeap Σ) : L :=
         List.fold_right (fun c h => ASS.inst_chunk ι c ∧ h) ltrue h.
-
-      (*   Definition rhoI {Γ Σ0} (ι0 : SymInstance Σ0) (s__sym : SymbolicState Γ Σ0) : *)
-      (*     Outcome (SCMutResult Γ { Σ : Ctx (𝑺 * Ty) & Sub Σ0 Σ * SymInstance Σ }%type) := *)
-      (*     ⨂ (Σ1 : Ctx (𝑺 * Ty)) *)
-      (*       (ζ1 : Sub Σ0 Σ1) *)
-      (*       (ι1 : SymInstance Σ1) *)
-      (*       (s__sc : SCState Γ) *)
-      (*       (_ : syminstance_rel ζ1 ι0 ι1) *)
-      (*       (_ : represents ι1 (subst ζ1 s__sym) s__sc) => *)
-      (*     outcome_pure *)
-      (*       {| scmutres_value := existT Σ1 (ζ1,ι1); *)
-      (*          scmutres_state := s__sc *)
-      (*       |}. *)
-      (* End Bla. *)
-
-      (* Definition approximates {Γ1 Γ2 Σ} (ι : SymInstance Σ) (dm : DynamicMutator Γ1 Γ2 Unit Σ) (sm : SCMut Γ1 Γ2 unit) : Prop. *)
-      (* Proof. *)
-      (*   refine ( *)
-      (*   forall s__sym : SymbolicState Γ1 Σ, *)
-      (*     outcome_cover *)
-      (*       (outcome_bind (dm Σ (sub_id _) s__sym) _) *)
-      (*       (outcome_bind (rhoI ι s__sym) (fun r__sc => sm (scmutres_state r__sc))) *)
-      (*     ). *)
-      (*   intros [Σ1 ζ1 [_ s__sym' x]]. *)
-      (*   eapply outcome_bind. *)
-      (*   eapply (rhoI ι). *)
-      (*   admit. *)
-      (*   intros [? s__sc']. *)
-      (*   apply outcome_pure. *)
-      (*   constructor. *)
-      (*   constructor. *)
-      (*   apply s__sc'. *)
-      (*   Show Proof. *)
 
       Ltac sauto :=
         repeat
@@ -542,15 +554,15 @@ Module Soundness
 
       Local Ltac sound_inster :=
         match goal with
-        | [ IH: SemiConcrete.Outcome.outcome_satisfy (dmut_exec ?s _ _) |-
-            SemiConcrete.Outcome.outcome_satisfy (dmut_exec ?s _ _) _ ] =>
-          refine (SemiConcrete.Outcome.outcome_satisfy_monotonic _ _ IH); clear IH
-        | [ IH: context[_ -> SemiConcrete.Outcome.outcome_satisfy (dmut_exec ?s _ _) _] |-
-            SemiConcrete.Outcome.outcome_satisfy (dmut_exec ?s _ _) _ ] =>
-          microsail_insterU (fail) IH; refine (SemiConcrete.Outcome.outcome_satisfy_monotonic _ _ IH); clear IH
+        | [ IH: outcome_satisfy (dmut_exec ?s _ _) |-
+            outcome_satisfy (dmut_exec ?s _ _) _ ] =>
+          refine (outcome_satisfy_monotonic _ _ IH); clear IH
+        | [ IH: context[_ -> outcome_satisfy (dmut_exec ?s _ _) _] |-
+            outcome_satisfy (dmut_exec ?s _ _) _ ] =>
+          microsail_insterU (fail) IH; refine (outcome_satisfy_monotonic _ _ IH); clear IH
         end.
 
-      Transparent SubstEnv.
+      Transparent subst SubstEnv.
       Lemma subst_lookup {Γ Σ Σ' x σ} (xInΓ : (x ∶ σ)%ctx ∈ Γ) (ζ : Sub Σ Σ') (δ : SymbolicLocalStore Γ Σ) :
         (subst ζ (δ ‼ x)%exp = (subst ζ δ ‼ x)%exp).
       Proof.
@@ -566,8 +578,7 @@ Module Soundness
         all: induction es; cbn in *; destruct_conjs; f_equal; auto.
       Qed.
 
-      Transparent inst.
-      Transparent instantiate_env.
+      Transparent inst instantiate_env.
 
       Lemma eval_exp_inst {Γ Σ τ} (ι : SymInstance Σ) (δΓΣ : SymbolicLocalStore Γ Σ) (e : Exp Γ τ) :
         eval e (inst ι δΓΣ) = inst ι (symbolic_eval_exp δΓΣ e).
@@ -598,7 +609,7 @@ Module Soundness
           let δ       := inst ι δ1 in
           let pre__pc   := inst_pathcondition ι pc1 in
           let pre__heap := interpret_heap ι h1 in
-          SemiConcrete.Outcome.outcome_satisfy
+          outcome_satisfy
             (dmut_exec s ζ1 (MkSymbolicState pc1 δ1 h1))
             (fun '(@MkDynMutResult _ _ _ Σ2 ζ2 t (MkSymbolicState pc2 δ2 h2)) =>
                forall (ι' : SymInstance Σ2),
@@ -607,7 +618,7 @@ Module Soundness
                  let post__heap := interpret_heap ι' h2 in
                  !! post__pc ∧ post__heap ⊢ POST (inst ι' t) (inst ι' δ2)) ->
           pre__pc ->
-          SemiConcrete.Outcome.outcome_satisfy
+          outcome_satisfy
             (scmut_exec s (MkSCState δ (inst ι h1)))
             (fun '(MkSCMutResult v2 (MkSCState δ2 h2)) =>
                SCMUT.inst_scheap h2 ⊢ POST v2 δ2).
@@ -650,7 +661,7 @@ Module Soundness
       Proof.
       Admitted.
 
-    End WithSemantics.
+    End  WithSemantics.
 
   End DynMutV1Soundness.
 
